Use real definitions in oset instead of overloads

osetScript.sml
@@ -12,42 +12,65 @@ val _ = temp_tight_equality ();
 val _ = type_abbrev ("oset", ``:('a,unit) balanced_map``);
 
 (* Basic definitions, that correspond directly to balanced tree operations *)
-val _ = overload_on ("good_oset", ``(\cmp s. good_cmp cmp ∧ invariant cmp s):('a -> 'a -> comparison) -> 'a oset -> bool``);
-val _ = overload_on ("oempty", ``empty:'a oset``);
-val _ = overload_on ("osingleton", ``(\v. singleton v ()):'a -> 'a oset``);
-val _ = overload_on ("oin", ``(\cmp v s. member cmp v s):('a -> 'a -> comparison) -> 'a -> 'a oset -> bool``);
-val _ = overload_on ("oinsert", ``(\cmp v s. insert cmp v () s):('a -> 'a -> comparison) -> 'a -> 'a oset -> 'a oset``);
-val _ = overload_on ("odelete", ``(\cmp s v. delete cmp v s):('a -> 'a -> comparison) -> 'a oset -> 'a -> 'a oset``);
-val _ = overload_on ("ounion", ``(\cmp s1 s2. union cmp s1 s2):('a -> 'a -> comparison) -> 'a oset -> 'a oset -> 'a oset``);
-val _ = overload_on ("oimage", ``(\cmp f s. map_keys cmp f s):('b -> 'b -> comparison) -> ('a -> 'b) -> 'a oset -> 'b oset``);
-val _ = overload_on ("osubset", ``(\cmp s1 s2. isSubmapOf cmp s1 s2):('a -> 'a -> comparison) -> 'a oset -> 'a oset -> bool``);
-val _ = overload_on ("ocompare", ``(\cmp s1 s2. compare (\(x,y) (x',y'). cmp x x') s1 s2):('a -> 'a -> comparison) -> 'a oset -> 'a oset -> comparison``);
-val _ = overload_on ("oevery", ``(\f s. every (\x y. f x) s):('a -> bool) -> 'a oset -> bool``);
-val _ = overload_on ("oexists", ``(\f s. exists (\x y. f x) s):('a -> bool) -> 'a oset -> bool``);
+val good_oset_def = Define `
+good_oset cmp (s:'a oset) ⇔ good_cmp cmp ∧ invariant cmp s`;
+
+val oempty_def = Define `
+oempty = empty:'a oset`;
+
+val osingleton_def = Define `
+osingleton v = singleton v ()`;
+
+val oin_def = Define `
+oin cmp (v:'a) (s:'a oset) ⇔  member cmp v s`;
+
+val oinsert_def = Define `
+oinsert cmp v s = insert cmp v () s`;
+
+val odelete_def = Define `
+odelete cmp (s:'a oset) (v:'a) = delete cmp v s`;
+
+val ounion_def = Define `
+ounion cmp (s1:'a oset) s2 = union cmp s1 s2`;
+
+val oimage_def = Define `
+oimage cmp f (s:'a oset) = map_keys cmp f s`;
+
+val osubset_def = Define `
+osubset cmp (s1:'a oset) (s2:'a oset) ⇔ isSubmapOf cmp s1 s2`;
+
+val ocompare_def = Define `
+ocompare cmp (s1:'a oset) (s2:'a oset) = compare (\(x,y) (x',y'). cmp x x') s1 s2`;
+
+val oevery_def = Define `
+oevery f (s:'a oset) ⇔  every (\x y. f x) s`;
+
+val oexists_def = Define `
+oexists f (s:'a oset) ⇔  exists (\x y. f x) s`;
 
 (* operations preserve good_set *)
 
 val good_oset_oempty = Q.store_thm ("good_oset_oempty",
 `!cmp. good_cmp cmp ⇒ good_oset cmp oempty`,
- rw [empty_thm]);
+ rw [empty_thm, good_oset_def, oempty_def]);
 
 val good_oset_singleton = Q.store_thm ("good_oset_singleton",
 `!cmp x. good_cmp cmp ⇒ good_oset cmp (osingleton x)`,
- rw [singleton_thm]);
+ rw [singleton_thm, good_oset_def, osingleton_def]);
 
 val good_oset_oinsert = Q.store_thm ("good_oset_oinsert",
 `!cmp s x. good_oset cmp s ⇒ good_oset cmp (oinsert cmp x s)`,
- rw [] >>
+ rw [oinsert_def, good_oset_def] >>
  metis_tac [insert_thm]);
 
 val good_oset_odelete = Q.store_thm ("good_oset_odelete",
 `!cmp s x. good_oset cmp s ⇒ good_oset cmp (odelete cmp s x)`,
- rw [] >>
+ rw [good_oset_def, odelete_def] >>
  metis_tac [delete_thm]);
 
 val good_oset_ounion = Q.store_thm ("good_oset_ounion",
 `!cmp s1 s2. good_oset cmp s1 ∧ good_oset cmp s2 ⇒ good_oset cmp (ounion cmp s1 s2)`,
- rw [] >>
+ rw [good_oset_def, ounion_def] >>
  metis_tac [union_thm]);
 
 val good_oset_oimage = Q.store_thm ("good_oset_oimage",
@@ -65,23 +88,23 @@ val good_cmp_ocompare = Q.store_thm ("good_cmp_ocompare",
  pop_assum (fn _ => all_tac) >>
  pop_assum (fn _ => all_tac) >>
  rw [] >>
- rw [good_cmp_def] >>
+ rw [ocompare_def, good_cmp_def] >>
  metis_tac [good_cmp_def]);
 
 (* How oin interacts with other operations *)
 
 val oin_oempty = Q.store_thm ("oin_oinsert",
 `!cmp x. oin cmp x oempty = F`,
- rw [empty_def, member_def]); 
+ rw [oin_def, oempty_def, empty_def, member_def]); 
 
 val oin_singleton = Q.store_thm ("oin_singleton",
 `∀cmp x y. oin cmp x (osingleton y) ⇔ cmp x y = Equal`,
- rw [member_def, singleton_def] >>
+ rw [oin_def, osingleton_def, member_def, singleton_def] >>
  EVERY_CASE_TAC);
 
 val oin_oinsert = Q.store_thm ("oin_oinsert",
 `∀cmp x y s. good_oset cmp s ⇒ (oin cmp x (oinsert cmp y s) ⇔ cmp x y = Equal ∨ oin cmp x s)`,
- rw [] >>
+ rw [good_oset_def, oin_def, oinsert_def] >>
  imp_res_tac insert_thm >>
  last_x_assum (qspecl_then [`()`, `y`] assume_tac) >>
  imp_res_tac member_thm >>
@@ -91,9 +114,10 @@ val oin_oinsert = Q.store_thm ("oin_oinsert",
 
 val oin_odelete = Q.store_thm ("oin_odelete",
 `!cmp s x y. good_oset cmp s ⇒ (oin cmp x (odelete cmp s y) ⇔ oin cmp x s ∧ cmp x y ≠ Equal)`,
- rw [] >>
+ rw [oin_def, odelete_def] >>
  imp_res_tac good_oset_odelete >>
  pop_assum (qspecl_then [`y`] assume_tac) >>
+ fs [good_oset_def, odelete_def] >>
  imp_res_tac delete_thm >>
  imp_res_tac member_thm >>
  rw [FDOM_DRESTRICT, key_set_eq] >>
@@ -102,8 +126,9 @@ val oin_odelete = Q.store_thm ("oin_odelete",
 
 val oin_ounion = Q.store_thm ("oin_ounion",
 `!cmp x s1 s2. good_oset cmp s1 ∧ good_oset cmp s2 ⇒ (oin cmp x (ounion cmp s1 s2) ⇔ oin cmp x s1 ∨ oin cmp x s2)`,
- rw [] >>
+ rw [oin_def] >>
  `good_oset cmp (ounion cmp s1 s2)` by metis_tac [good_oset_ounion] >>
+ fs [good_oset_def, ounion_def] >>
  imp_res_tac member_thm >>
  rw [] >>
  `to_fmap cmp (union cmp s1 s2) = to_fmap cmp s1 ⊌ to_fmap cmp s2` by metis_tac [union_thm] >>
@@ -127,7 +152,7 @@ val oevery_oin = Q.store_thm ("oevery_oin",
   (∀k1 k2. cmp k1 k2 = Equal ⇒ (f k1 ⇔ f k2))
   ⇒ 
   (oevery f s ⇔ (!x. oin cmp x s ⇒ f x))`,
- rw [] >>
+ rw [good_oset_def, oevery_def, oin_def] >>
  `∀k1 (v:unit) k2 (v:unit). cmp k1 k2 = Equal ⇒ ((\x y. f x) k1 v ⇔ (\x y. f x) k2 v)` by metis_tac [] >>
  imp_res_tac every_thm >>
  rw [lookup_thm, flookup_thm, member_thm]);
@@ -138,7 +163,7 @@ val oexists_oin = Q.store_thm ("oexists_oin",
   (∀k1 k2. cmp k1 k2 = Equal ⇒ (f k1 ⇔ f k2))
   ⇒ 
   (oexists f s ⇔ (?x. oin cmp x s ∧ f x))`,
- rw [] >>
+ rw [good_oset_def, oexists_def, oin_def] >>
  `∀k1 (v:unit) k2 (v:unit). cmp k1 k2 = Equal ⇒ ((\x y. f x) k1 v ⇔ (\x y. f x) k2 v)` by metis_tac [] >>
  imp_res_tac exists_thm >>
  rw [lookup_thm, flookup_thm, member_thm]);
